IOAPIC definition and show that output port is bound
Signed-off-by: Lukas Humbel <lukas.humbel@inf.ethz.ch>

theories/interrupt/x86int.thy
@@ -36,7 +36,7 @@ SOFTWARE, EVEN IF ADVISED OF THE POSSIBILITY OF SUCH DAMAGE.
 
 theory x86int
 imports
-  interrupt Main Set
+  interrupt Main "HOL-Word.Word" "HOL-Word.WordBitwise"
 begin
 
 (* Delivery Mode *)
@@ -45,6 +45,68 @@ datatype DLM = DLMFIXED  | DLMLOWPRIO | DLMSMI | DLMNMI | DLMINIT | DLMEXTINT
 (* Destination Mode *)
 datatype DM = DMPHYS | DMLOGICAL
 
-  
+(* Trigger Mode *)
+datatype TRIGGERM = TRIGGERMEDGE | TRIGGERMLEVEL
 
+type_synonym word8 = "8 word"
+type_synonym word4 = "4 word"
+
+(* Encode Destination mode and the dest field (the dest field interpretation
+   depends on the destination mode *)
+datatype DMDEST = DMPHYS word4 | DMLOGICAL word8
+
+(* IOAPIC Redirection table entry, see 82093AA Datasheet *)
+record IOREDTBL_ENTRY =
+  dest :: DMDEST
+  mask :: bool
+  trigger :: TRIGGERM
+  delmode :: DLM
+  remote_irr :: bool (* Read only *)
+  intpol_high :: bool (* true=active high *)
+  delivs :: bool (* Read only *)
+  vector :: nat
+
+(* This is for the original IOAPIC that has an 8 bit destination *)
+definition ioredtbl_entry_well_formed :: "IOREDTBL_ENTRY \<Rightarrow> bool"
+  where "ioredtbl_entry_well_formed iot \<longleftrightarrow> (vector iot) < 256"
+
+definition tset :: "nat set"
+  where "tset = {}"
+
+definition to_indexset :: "word8 \<Rightarrow> nat set"
+  where "to_indexset w = {x. (w !! x) }"
+
+lemma "to_indexset 255 = {7,6,5,4,3,2,1,0}"
+  using bin_nth_Bit0 bin_nth_Bit1 by (simp add:to_indexset_def, auto)
+
+lemma bit_set_bound: "w !! n \<longrightarrow> n < 8"
+  for w :: "8 word"
+proof -
+  have L1: "size w \<le> 8"
+    by(simp only:word_size, auto)
+
+  have L2: "w !! n \<longrightarrow> n < size w"
+    by(simp add:test_bit_size)
+
+  show ?thesis
+    using L1 L2 less_trans by auto
+qed
+
+lemma to_indexset_bound: "\<forall> inp. to_indexset inp \<subseteq> {x. x < 8}"
+  using bit_set_bound by (simp add: to_indexset_def, auto)
+  
+(* Turns a IOREDTBL_ENTRY at index i to a IRQ, Source: Intel 10.6.2.1 *)
+definition ioredtbl_entry_to_irq_dest :: "IOREDTBL_ENTRY \<Rightarrow> IRQ set"
+  where "ioredtbl_entry_to_irq_dest iot = (case (dest iot) of
+    DMPHYS x \<Rightarrow> { \<lparr>format = FVECTOR (vector iot), port = unat x\<rparr> } |
+    DMLOGICAL ldest \<Rightarrow> {x.\<exists>y \<in> (to_indexset ldest). x = \<lparr> format = FVECTOR (vector iot), port = y \<rparr>})"
+
+(* In physical destination mode, the IOAPIC can address a 4 bit destination *)  
+lemma "\<forall>outi \<in> (ioredtbl_entry_to_irq_dest y). (port outi) < 16"
+  apply(case_tac "dest y")
+   apply(simp add:ioredtbl_entry_to_irq_dest_def, unat_arith, auto)
+  apply(simp add:ioredtbl_entry_to_irq_dest_def)
+  apply(auto)
+  using bit_set_bound to_indexset_def by fastforce
+    
 end
