theories/interrupt/lapic.thy
@@ -1,0 +1,50 @@
+(*
+
+Copyright (c) 2017, 2018, ETH Zurich
+All rights reserved.
+
+Redistribution and use in source and binary forms, with or without
+modification, are permitted provided that the following conditions are met:
+
+1. Redistributions of source code must retain the above copyright notice, this
+   list of conditions and the following disclaimer.
+2. Redistributions in binary form must reproduce the above copyright notice,
+   this list of conditions and the following disclaimer in the documentation
+   and/or other materials provided with the distribution.
+
+THIS SOFTWARE IS PROVIDED BY THE COPYRIGHT HOLDERS AND CONTRIBUTORS "AS IS" AND
+ANY EXPRESS OR IMPLIED WARRANTIES, INCLUDING, BUT NOT LIMITED TO, THE IMPLIED
+WARRANTIES OF MERCHANTABILITY AND FITNESS FOR A PARTICULAR PURPOSE ARE
+DISCLAIMED. IN NO EVENT SHALL THE COPYRIGHT OWNER OR CONTRIBUTORS BE LIABLE FOR
+ANY DIRECT, INDIRECT, INCIDENTAL, SPECIAL, EXEMPLARY, OR CONSEQUENTIAL DAMAGES
+(INCLUDING, BUT NOT LIMITED TO, PROCUREMENT OF SUBSTITUTE GOODS OR SERVICES;
+LOSS OF USE, DATA, OR PROFITS; OR BUSINESS INTERRUPTION) HOWEVER CAUSED AND
+ON ANY THEORY OF LIABILITY, WHETHER IN CONTRACT, STRICT LIABILITY, OR TORT
+(INCLUDING NEGLIGENCE OR OTHERWISE) ARISING IN ANY WAY OUT OF THE USE OF THIS
+SOFTWARE, EVEN IF ADVISED OF THE POSSIBILITY OF SUCH DAMAGE.
+
+*)
+
+(*<*)
+theory lapic
+  imports interrupt x86int "HOL-Word.Word" "HOL-Word.WordBitwise"
+begin
+(*>*)
+
+datatype DFR = DFRFLAT | DFRCLUSTER
+
+type_synonym word8 = "8 word"
+
+record LAPIC =
+  id :: nat (* Hardware given, physical APIC ID *)
+  ldr :: word8 (* Logical destination register *)
+  dfr :: DFR (* Destination Format Register *)
+
+(* Local vector table entry *)
+record LVT =
+  delivery :: DLM
+  mask :: bool
+
+(* In LVT entries, lowprio is DLM is not allowed *)
+definition lapic_lvt_well_formed :: "LVT \<Rightarrow> bool"
+  where "lapic_lvt_well_formed x \<longleftrightarrow> (delivery x) \<noteq> DLMLOWPRIO"
